HOL-ETCS/Equalizer.thy
@@ -1,8 +1,8 @@
+section \<open>Equalizers and Subobjects\<close>
+
 theory Equalizer
   imports Terminal
 begin
-
-section \<open>Equalizers and Subobjects\<close>
 
 subsection \<open>Equalizers\<close>
 
@@ -270,70 +270,7 @@ proof auto
     by (rule_tac x="k \<circ>\<^sub>c a" in exI, auto)
 qed
 
-section \<open>Pullback\<close>
-
-text \<open>The definition below corresponds to a definition stated between Definition 2.1.42 and Definition 2.1.43 in Halvorson.\<close>
-definition is_pullback :: "cset \<Rightarrow> cset \<Rightarrow> cset \<Rightarrow> cset \<Rightarrow> cfunc \<Rightarrow> cfunc \<Rightarrow> cfunc \<Rightarrow> cfunc \<Rightarrow> bool" where
-  "is_pullback A B C D ab bd ac cd \<longleftrightarrow> 
-    (ab : A \<rightarrow> B \<and> bd : B \<rightarrow> D \<and> ac : A \<rightarrow> C \<and> cd : C \<rightarrow> D \<and> bd \<circ>\<^sub>c ab = cd \<circ>\<^sub>c ac \<and> 
-    (\<forall> Z k h. (k : Z \<rightarrow> B \<and> h : Z \<rightarrow> C \<and> bd \<circ>\<^sub>c k = cd \<circ>\<^sub>c h)  \<longrightarrow>
-      (\<exists>! j. j : Z \<rightarrow> A \<and> ab \<circ>\<^sub>c j = k \<and> ac \<circ>\<^sub>c j = h)))"
-
-lemma pullback_iff_product:
-  assumes "terminal_object(T)"
-  assumes f_type[type_rule]: "f : Y \<rightarrow> T" 
-  assumes g_type[type_rule]: "g : X \<rightarrow> T"
-  shows "(is_pullback P Y X T (pY) f (pX) g) = (is_cart_prod P pX pY X Y)"
-proof(auto)
-  assume pullback: "is_pullback P Y X T pY f pX g"
-  have f_type[type_rule]: "f : Y \<rightarrow> T"
-    using is_pullback_def pullback by force
-  have g_type[type_rule]: "g : X \<rightarrow> T"
-    using is_pullback_def pullback by force
-  show "is_cart_prod P pX pY X Y"
-  proof(unfold is_cart_prod_def, auto)
-    show pX_type[type_rule]: "pX : P \<rightarrow> X"
-      using pullback is_pullback_def by force
-    show pY_type[type_rule]: "pY : P \<rightarrow> Y"
-      using pullback is_pullback_def by force
-    show "\<And>x y Z.
-       x : Z \<rightarrow> X \<Longrightarrow>
-       y : Z \<rightarrow> Y \<Longrightarrow>
-       \<exists>h. h : Z \<rightarrow> P \<and>
-           pX \<circ>\<^sub>c h = x \<and> pY \<circ>\<^sub>c h = y \<and> (\<forall>h2. h2 : Z \<rightarrow> P \<and> pX \<circ>\<^sub>c h2 = x \<and> pY \<circ>\<^sub>c h2 = y \<longrightarrow> h2 = h)"
-    proof - 
-      fix x y Z
-      assume x_type[type_rule]: "x : Z \<rightarrow> X"
-      assume y_type[type_rule]: "y : Z \<rightarrow> Y"
-      have  "\<And>Z k h. k : Z \<rightarrow> Y \<Longrightarrow> h : Z \<rightarrow> X \<Longrightarrow> f \<circ>\<^sub>c k = g \<circ>\<^sub>c h \<Longrightarrow> \<exists>j. j : Z \<rightarrow> P \<and> pY \<circ>\<^sub>c j = k \<and> pX \<circ>\<^sub>c j = h"
-        using is_pullback_def pullback by blast
-      then have "\<exists>h. h : Z \<rightarrow> P \<and>
-           pX \<circ>\<^sub>c h = x \<and> pY \<circ>\<^sub>c h = y"
-        by (smt (verit, ccfv_threshold) assms cfunc_type_def codomain_comp domain_comp f_type g_type terminal_object_def x_type y_type)
-      then show "\<exists>h. h : Z \<rightarrow> P \<and>
-           pX \<circ>\<^sub>c h = x \<and> pY \<circ>\<^sub>c h = y \<and> (\<forall>h2. h2 : Z \<rightarrow> P \<and> pX \<circ>\<^sub>c h2 = x \<and> pY \<circ>\<^sub>c h2 = y \<longrightarrow> h2 = h)"
-        by (typecheck_cfuncs, smt (verit, ccfv_threshold) comp_associative2 is_pullback_def pullback)
-    qed
-  qed
-next
-  assume prod: "is_cart_prod P pX pY X Y"
-  then show "is_pullback P Y X T pY f pX g"
-  proof(unfold is_cart_prod_def is_pullback_def, typecheck_cfuncs, auto)
-    assume pX_type[type_rule]: "pX : P \<rightarrow> X"
-    assume pY_type[type_rule]: "pY : P \<rightarrow> Y"
-    show "f \<circ>\<^sub>c pY = g \<circ>\<^sub>c pX"
-      using assms(1) terminal_object_def by (typecheck_cfuncs, auto)  
-    show "\<And>Z k h. k : Z \<rightarrow> Y \<Longrightarrow> h : Z \<rightarrow> X \<Longrightarrow> f \<circ>\<^sub>c k = g \<circ>\<^sub>c h \<Longrightarrow> \<exists>j. j : Z \<rightarrow> P \<and> pY \<circ>\<^sub>c j = k \<and> pX \<circ>\<^sub>c j = h"
-      using is_cart_prod_def prod by blast
-    show "\<And>Z j y.
-       pY \<circ>\<^sub>c j : Z \<rightarrow> Y \<Longrightarrow>
-       pX \<circ>\<^sub>c j : Z \<rightarrow> X \<Longrightarrow>
-       f \<circ>\<^sub>c pY \<circ>\<^sub>c j = g \<circ>\<^sub>c pX \<circ>\<^sub>c j \<Longrightarrow> j : Z \<rightarrow> P \<Longrightarrow> y : Z \<rightarrow> P \<Longrightarrow> pY \<circ>\<^sub>c y = pY \<circ>\<^sub>c j \<Longrightarrow> pX \<circ>\<^sub>c y = pX \<circ>\<^sub>c j \<Longrightarrow> j = y"
-      using is_cart_prod_def prod by blast
-  qed
-qed
-
-section \<open>Inverse Image\<close>
+subsection \<open>Inverse Image\<close>
 
 text\<open>The definition below corresponds to a definition given by a diagram between Definition 2.1.37 and Proposition 2.1.38 in Halvorson.\<close>
 definition inverse_image :: "cfunc \<Rightarrow> cset \<Rightarrow> cfunc \<Rightarrow> cset" ("_\<^sup>-\<^sup>1\<lparr>_\<rparr>\<^bsub>_\<^esub>" [101,0,0]100) where
@@ -550,7 +487,7 @@ next
     by (typecheck_cfuncs, simp add: inverse_image_monomorphism)
 qed
 
-section \<open>Fibered Products\<close>
+subsection \<open>Fibered Products\<close>
 
 text \<open>The definition below corresponds to Definition 2.1.42 in Halvorson.\<close>
 definition fibered_product :: "cset \<Rightarrow> cfunc \<Rightarrow> cfunc \<Rightarrow> cset \<Rightarrow> cset" ("_ \<^bsub>_\<^esub>\<times>\<^sub>c\<^bsub>_\<^esub> _" [66,50,50,65]65) where
