HOL-ETCS/Cardinality.thy
@@ -1,8 +1,8 @@
+section \<open>Cardinality and Finiteness\<close>
+
 theory Cardinality
   imports Exponential_Objects
 begin
-
-section \<open>Cardinality and Finiteness\<close>
 
 text \<open>The definitions below correspond to Definition 2.6.1 in Halvorson.\<close>
 definition is_finite :: "cset \<Rightarrow> bool"  where
@@ -572,7 +572,7 @@ next
         assume "\<not> terminal_object X"
 
         obtain into where into_def: "into = (left_cart_proj Y one \<amalg> ((y2 \<amalg> y1) \<circ>\<^sub>c case_bool \<circ>\<^sub>c eq_pred Y \<circ>\<^sub>c (id Y \<times>\<^sub>f y1))) 
-                               \<circ>\<^sub>c dist_prod_coprod_inv Y one one \<circ>\<^sub>c (id Y \<times>\<^sub>f case_bool) \<circ>\<^sub>c (id Y \<times>\<^sub>f eq_pred X) "
+                               \<circ>\<^sub>c dist_prod_coprod_left Y one one \<circ>\<^sub>c (id Y \<times>\<^sub>f case_bool) \<circ>\<^sub>c (id Y \<times>\<^sub>f eq_pred X) "
           by simp
         then have into_type[type_rule]: "into : Y \<times>\<^sub>c (X \<times>\<^sub>c X) \<rightarrow> Y"
           by (simp, typecheck_cfuncs)
@@ -633,23 +633,23 @@ next
           have "(\<Theta> \<circ>\<^sub>c \<langle>x, y\<rangle>)\<^sup>\<flat> \<circ>\<^sub>c \<langle>id X, \<beta>\<^bsub>X\<^esub>\<rangle> \<circ>\<^sub>c x = into \<circ>\<^sub>c   \<langle>y, \<langle>x, x\<rangle>\<rangle>"
             by (simp add: f0 x_type y_type)
           also have "... = (left_cart_proj Y one \<amalg> ((y2 \<amalg> y1) \<circ>\<^sub>c case_bool \<circ>\<^sub>c eq_pred Y \<circ>\<^sub>c (id Y \<times>\<^sub>f y1)))
-                                 \<circ>\<^sub>c dist_prod_coprod_inv Y one one \<circ>\<^sub>c (id Y \<times>\<^sub>f case_bool) \<circ>\<^sub>c (id Y \<times>\<^sub>f eq_pred X) \<circ>\<^sub>c   \<langle>y, \<langle>x, x\<rangle>\<rangle>"
+                                 \<circ>\<^sub>c dist_prod_coprod_left Y one one \<circ>\<^sub>c (id Y \<times>\<^sub>f case_bool) \<circ>\<^sub>c (id Y \<times>\<^sub>f eq_pred X) \<circ>\<^sub>c   \<langle>y, \<langle>x, x\<rangle>\<rangle>"
             using cfunc_type_def comp_associative comp_type into_def by (typecheck_cfuncs, fastforce)
           also have "... = (left_cart_proj Y one \<amalg> ((y2 \<amalg> y1) \<circ>\<^sub>c case_bool \<circ>\<^sub>c eq_pred Y \<circ>\<^sub>c (id Y \<times>\<^sub>f y1)))
-                                 \<circ>\<^sub>c dist_prod_coprod_inv Y one one \<circ>\<^sub>c (id Y \<times>\<^sub>f case_bool) \<circ>\<^sub>c  \<langle>id Y \<circ>\<^sub>c y, eq_pred X \<circ>\<^sub>c  \<langle>x, x\<rangle>\<rangle>"
+                                 \<circ>\<^sub>c dist_prod_coprod_left Y one one \<circ>\<^sub>c (id Y \<times>\<^sub>f case_bool) \<circ>\<^sub>c  \<langle>id Y \<circ>\<^sub>c y, eq_pred X \<circ>\<^sub>c  \<langle>x, x\<rangle>\<rangle>"
             by (typecheck_cfuncs, simp add: cfunc_cross_prod_comp_cfunc_prod)
          also have "... = (left_cart_proj Y one \<amalg> ((y2 \<amalg> y1) \<circ>\<^sub>c case_bool \<circ>\<^sub>c eq_pred Y \<circ>\<^sub>c (id Y \<times>\<^sub>f y1))) 
-                                 \<circ>\<^sub>c dist_prod_coprod_inv Y one one \<circ>\<^sub>c (id Y \<times>\<^sub>f case_bool) \<circ>\<^sub>c  \<langle>y, \<t>\<rangle>"
+                                 \<circ>\<^sub>c dist_prod_coprod_left Y one one \<circ>\<^sub>c (id Y \<times>\<^sub>f case_bool) \<circ>\<^sub>c  \<langle>y, \<t>\<rangle>"
             by (typecheck_cfuncs, metis eq_pred_iff_eq id_left_unit2)
           also have "... = (left_cart_proj Y one \<amalg> ((y2 \<amalg> y1) \<circ>\<^sub>c case_bool \<circ>\<^sub>c eq_pred Y \<circ>\<^sub>c (id Y \<times>\<^sub>f y1))) 
-                                 \<circ>\<^sub>c dist_prod_coprod_inv Y one one  \<circ>\<^sub>c  \<langle>y, left_coproj one one\<rangle>"
+                                 \<circ>\<^sub>c dist_prod_coprod_left Y one one  \<circ>\<^sub>c  \<langle>y, left_coproj one one\<rangle>"
             by (typecheck_cfuncs, simp add: case_bool_true cfunc_cross_prod_comp_cfunc_prod id_left_unit2)
           also have "... = (left_cart_proj Y one \<amalg> ((y2 \<amalg> y1) \<circ>\<^sub>c case_bool \<circ>\<^sub>c eq_pred Y \<circ>\<^sub>c (id Y \<times>\<^sub>f y1))) 
-                                 \<circ>\<^sub>c dist_prod_coprod_inv Y one one  \<circ>\<^sub>c  \<langle>y, left_coproj one one \<circ>\<^sub>c id one\<rangle>"
+                                 \<circ>\<^sub>c dist_prod_coprod_left Y one one  \<circ>\<^sub>c  \<langle>y, left_coproj one one \<circ>\<^sub>c id one\<rangle>"
             by (typecheck_cfuncs, metis id_right_unit2)
           also have "... = (left_cart_proj Y one \<amalg> ((y2 \<amalg> y1) \<circ>\<^sub>c case_bool \<circ>\<^sub>c eq_pred Y \<circ>\<^sub>c (id Y \<times>\<^sub>f y1))) 
                                  \<circ>\<^sub>c left_coproj (Y \<times>\<^sub>c one) (Y \<times>\<^sub>c one) \<circ>\<^sub>c \<langle>y,id one\<rangle>"
-            using dist_prod_coprod_inv_left_ap by (typecheck_cfuncs, presburger)
+            using dist_prod_coprod_left_ap_left by (typecheck_cfuncs, presburger)
           also have "... = ((left_cart_proj Y one \<amalg> ((y2 \<amalg> y1) \<circ>\<^sub>c case_bool \<circ>\<^sub>c eq_pred Y \<circ>\<^sub>c (id Y \<times>\<^sub>f y1))) 
                                  \<circ>\<^sub>c left_coproj (Y \<times>\<^sub>c one) (Y \<times>\<^sub>c one)) \<circ>\<^sub>c \<langle>y,id one\<rangle>"
             by (typecheck_cfuncs, meson comp_associative2)
@@ -672,23 +672,23 @@ next
           have "(\<Theta> \<circ>\<^sub>c \<langle>x, y\<rangle>)\<^sup>\<flat> \<circ>\<^sub>c \<langle>id X, \<beta>\<^bsub>X\<^esub>\<rangle> \<circ>\<^sub>c z = into \<circ>\<^sub>c   \<langle>y, \<langle>x, z\<rangle>\<rangle>"
             by (simp add: f0 x_type y_type z_type)
           also have "... = (left_cart_proj Y one \<amalg> ((y2 \<amalg> y1) \<circ>\<^sub>c case_bool \<circ>\<^sub>c eq_pred Y \<circ>\<^sub>c (id Y \<times>\<^sub>f y1)))
-                                 \<circ>\<^sub>c dist_prod_coprod_inv Y one one \<circ>\<^sub>c (id Y \<times>\<^sub>f case_bool) \<circ>\<^sub>c (id Y \<times>\<^sub>f eq_pred X) \<circ>\<^sub>c   \<langle>y, \<langle>x, z\<rangle>\<rangle>"
+                                 \<circ>\<^sub>c dist_prod_coprod_left Y one one \<circ>\<^sub>c (id Y \<times>\<^sub>f case_bool) \<circ>\<^sub>c (id Y \<times>\<^sub>f eq_pred X) \<circ>\<^sub>c   \<langle>y, \<langle>x, z\<rangle>\<rangle>"
             using cfunc_type_def comp_associative comp_type into_def by (typecheck_cfuncs, fastforce)
           also have "... = (left_cart_proj Y one \<amalg> ((y2 \<amalg> y1) \<circ>\<^sub>c case_bool \<circ>\<^sub>c eq_pred Y \<circ>\<^sub>c (id Y \<times>\<^sub>f y1)))
-                                 \<circ>\<^sub>c dist_prod_coprod_inv Y one one \<circ>\<^sub>c (id Y \<times>\<^sub>f case_bool) \<circ>\<^sub>c  \<langle>id Y \<circ>\<^sub>c y, eq_pred X \<circ>\<^sub>c  \<langle>x, z\<rangle>\<rangle>"
+                                 \<circ>\<^sub>c dist_prod_coprod_left Y one one \<circ>\<^sub>c (id Y \<times>\<^sub>f case_bool) \<circ>\<^sub>c  \<langle>id Y \<circ>\<^sub>c y, eq_pred X \<circ>\<^sub>c  \<langle>x, z\<rangle>\<rangle>"
             by (typecheck_cfuncs, simp add: cfunc_cross_prod_comp_cfunc_prod)
           also have "... = (left_cart_proj Y one \<amalg> ((y2 \<amalg> y1) \<circ>\<^sub>c case_bool \<circ>\<^sub>c eq_pred Y \<circ>\<^sub>c (id Y \<times>\<^sub>f y1))) 
-                                 \<circ>\<^sub>c dist_prod_coprod_inv Y one one \<circ>\<^sub>c (id Y \<times>\<^sub>f case_bool) \<circ>\<^sub>c  \<langle>y, \<f>\<rangle>"
+                                 \<circ>\<^sub>c dist_prod_coprod_left Y one one \<circ>\<^sub>c (id Y \<times>\<^sub>f case_bool) \<circ>\<^sub>c  \<langle>y, \<f>\<rangle>"
             by (typecheck_cfuncs, metis \<open>z \<noteq> x\<close> eq_pred_iff_eq_conv id_left_unit2)
           also have "... = (left_cart_proj Y one \<amalg> ((y2 \<amalg> y1) \<circ>\<^sub>c case_bool \<circ>\<^sub>c eq_pred Y \<circ>\<^sub>c (id Y \<times>\<^sub>f y1))) 
-                                 \<circ>\<^sub>c dist_prod_coprod_inv Y one one  \<circ>\<^sub>c  \<langle>y, right_coproj one one\<rangle>"
+                                 \<circ>\<^sub>c dist_prod_coprod_left Y one one  \<circ>\<^sub>c  \<langle>y, right_coproj one one\<rangle>"
             by (typecheck_cfuncs, simp add: case_bool_false cfunc_cross_prod_comp_cfunc_prod id_left_unit2)
           also have "... = (left_cart_proj Y one \<amalg> ((y2 \<amalg> y1) \<circ>\<^sub>c case_bool \<circ>\<^sub>c eq_pred Y \<circ>\<^sub>c (id Y \<times>\<^sub>f y1)))
-                                 \<circ>\<^sub>c dist_prod_coprod_inv Y one one  \<circ>\<^sub>c  \<langle>y, right_coproj one one \<circ>\<^sub>c id one\<rangle>"
+                                 \<circ>\<^sub>c dist_prod_coprod_left Y one one  \<circ>\<^sub>c  \<langle>y, right_coproj one one \<circ>\<^sub>c id one\<rangle>"
             by (typecheck_cfuncs, simp add: id_right_unit2)
           also have "... = (left_cart_proj Y one \<amalg> ((y2 \<amalg> y1) \<circ>\<^sub>c case_bool \<circ>\<^sub>c eq_pred Y \<circ>\<^sub>c (id Y \<times>\<^sub>f y1)))
                                  \<circ>\<^sub>c right_coproj (Y \<times>\<^sub>c one) (Y \<times>\<^sub>c one) \<circ>\<^sub>c \<langle>y,id one\<rangle>"
-            using dist_prod_coprod_inv_right_ap by (typecheck_cfuncs, presburger)
+            using dist_prod_coprod_left_ap_right by (typecheck_cfuncs, presburger)
           also have "... = ((left_cart_proj Y one \<amalg> ((y2 \<amalg> y1) \<circ>\<^sub>c case_bool \<circ>\<^sub>c eq_pred Y \<circ>\<^sub>c (id Y \<times>\<^sub>f y1))) 
                                  \<circ>\<^sub>c right_coproj (Y \<times>\<^sub>c one) (Y \<times>\<^sub>c one)) \<circ>\<^sub>c \<langle>y,id one\<rangle>"
             by (typecheck_cfuncs, meson comp_associative2)
@@ -718,23 +718,23 @@ next
           have "(\<Theta> \<circ>\<^sub>c \<langle>x, y1\<rangle>)\<^sup>\<flat> \<circ>\<^sub>c \<langle>id X, \<beta>\<^bsub>X\<^esub>\<rangle> \<circ>\<^sub>c z = into \<circ>\<^sub>c   \<langle>y1, \<langle>x, z\<rangle>\<rangle>"
             by (simp add: f0 x_type y1_type z_type)
           also have "... = (left_cart_proj Y one \<amalg> ((y2 \<amalg> y1) \<circ>\<^sub>c case_bool \<circ>\<^sub>c eq_pred Y \<circ>\<^sub>c (id Y \<times>\<^sub>f y1)))
-                                 \<circ>\<^sub>c dist_prod_coprod_inv Y one one \<circ>\<^sub>c (id Y \<times>\<^sub>f case_bool) \<circ>\<^sub>c (id Y \<times>\<^sub>f eq_pred X) \<circ>\<^sub>c   \<langle>y1, \<langle>x, z\<rangle>\<rangle>"
+                                 \<circ>\<^sub>c dist_prod_coprod_left Y one one \<circ>\<^sub>c (id Y \<times>\<^sub>f case_bool) \<circ>\<^sub>c (id Y \<times>\<^sub>f eq_pred X) \<circ>\<^sub>c   \<langle>y1, \<langle>x, z\<rangle>\<rangle>"
             using cfunc_type_def comp_associative comp_type into_def by (typecheck_cfuncs, fastforce)
           also have "... = (left_cart_proj Y one \<amalg> ((y2 \<amalg> y1) \<circ>\<^sub>c case_bool \<circ>\<^sub>c eq_pred Y \<circ>\<^sub>c (id Y \<times>\<^sub>f y1)))
-                                 \<circ>\<^sub>c dist_prod_coprod_inv Y one one \<circ>\<^sub>c (id Y \<times>\<^sub>f case_bool) \<circ>\<^sub>c  \<langle>id Y \<circ>\<^sub>c y1, eq_pred X \<circ>\<^sub>c  \<langle>x, z\<rangle>\<rangle>"
+                                 \<circ>\<^sub>c dist_prod_coprod_left Y one one \<circ>\<^sub>c (id Y \<times>\<^sub>f case_bool) \<circ>\<^sub>c  \<langle>id Y \<circ>\<^sub>c y1, eq_pred X \<circ>\<^sub>c  \<langle>x, z\<rangle>\<rangle>"
             by (typecheck_cfuncs, simp add: cfunc_cross_prod_comp_cfunc_prod)
           also have "... = (left_cart_proj Y one \<amalg> ((y2 \<amalg> y1) \<circ>\<^sub>c case_bool \<circ>\<^sub>c eq_pred Y \<circ>\<^sub>c (id Y \<times>\<^sub>f y1))) 
-                                 \<circ>\<^sub>c dist_prod_coprod_inv Y one one \<circ>\<^sub>c (id Y \<times>\<^sub>f case_bool) \<circ>\<^sub>c  \<langle>y1, \<f>\<rangle>"
+                                 \<circ>\<^sub>c dist_prod_coprod_left Y one one \<circ>\<^sub>c (id Y \<times>\<^sub>f case_bool) \<circ>\<^sub>c  \<langle>y1, \<f>\<rangle>"
             by (typecheck_cfuncs, metis \<open>z \<noteq> x\<close> eq_pred_iff_eq_conv id_left_unit2)
           also have "... = (left_cart_proj Y one \<amalg> ((y2 \<amalg> y1) \<circ>\<^sub>c case_bool \<circ>\<^sub>c eq_pred Y \<circ>\<^sub>c (id Y \<times>\<^sub>f y1))) 
-                                 \<circ>\<^sub>c dist_prod_coprod_inv Y one one  \<circ>\<^sub>c  \<langle>y1, right_coproj one one\<rangle>"
+                                 \<circ>\<^sub>c dist_prod_coprod_left Y one one  \<circ>\<^sub>c  \<langle>y1, right_coproj one one\<rangle>"
             by (typecheck_cfuncs, simp add: case_bool_false cfunc_cross_prod_comp_cfunc_prod id_left_unit2)
           also have "... = (left_cart_proj Y one \<amalg> ((y2 \<amalg> y1) \<circ>\<^sub>c case_bool \<circ>\<^sub>c eq_pred Y \<circ>\<^sub>c (id Y \<times>\<^sub>f y1)))
-                                 \<circ>\<^sub>c dist_prod_coprod_inv Y one one  \<circ>\<^sub>c  \<langle>y1, right_coproj one one \<circ>\<^sub>c id one\<rangle>"
+                                 \<circ>\<^sub>c dist_prod_coprod_left Y one one  \<circ>\<^sub>c  \<langle>y1, right_coproj one one \<circ>\<^sub>c id one\<rangle>"
             by (typecheck_cfuncs, simp add: id_right_unit2)
           also have "... = (left_cart_proj Y one \<amalg> ((y2 \<amalg> y1) \<circ>\<^sub>c case_bool \<circ>\<^sub>c eq_pred Y \<circ>\<^sub>c (id Y \<times>\<^sub>f y1)))
                                  \<circ>\<^sub>c right_coproj (Y \<times>\<^sub>c one) (Y \<times>\<^sub>c one) \<circ>\<^sub>c \<langle>y1,id one\<rangle>"
-            using dist_prod_coprod_inv_right_ap by (typecheck_cfuncs, presburger)
+            using dist_prod_coprod_left_ap_right by (typecheck_cfuncs, presburger)
           also have "... = ((left_cart_proj Y one \<amalg> ((y2 \<amalg> y1) \<circ>\<^sub>c case_bool \<circ>\<^sub>c eq_pred Y \<circ>\<^sub>c (id Y \<times>\<^sub>f y1))) 
                                  \<circ>\<^sub>c right_coproj (Y \<times>\<^sub>c one) (Y \<times>\<^sub>c one)) \<circ>\<^sub>c \<langle>y1,id one\<rangle>"
             by (typecheck_cfuncs, meson comp_associative2)
@@ -969,25 +969,25 @@ proof (unfold is_smaller_than_def)
 
   show "\<exists>m. m : X\<^bsup>A\<^esup> \<rightarrow> X\<^bsup>B\<^esup> \<and> monomorphism m"
   proof (rule_tac x="(((eval_func X A \<circ>\<^sub>c swap (X\<^bsup>A\<^esup>) A) \<amalg> (x \<circ>\<^sub>c \<beta>\<^bsub>X\<^bsup>A\<^esup> \<times>\<^sub>c (B \<setminus> (A, m))\<^esub>))
-    \<circ>\<^sub>c dist_prod_coprod_inv (X\<^bsup>A\<^esup>) A (B \<setminus> (A, m)) 
+    \<circ>\<^sub>c dist_prod_coprod_left (X\<^bsup>A\<^esup>) A (B \<setminus> (A, m)) 
     \<circ>\<^sub>c swap (A \<Coprod> (B \<setminus> (A, m))) (X\<^bsup>A\<^esup>) \<circ>\<^sub>c (try_cast m \<times>\<^sub>f id (X\<^bsup>A\<^esup>)))\<^sup>\<sharp>" in exI, auto)
 
-    show "((eval_func X A \<circ>\<^sub>c swap (X\<^bsup>A\<^esup>) A) \<amalg> (x \<circ>\<^sub>c \<beta>\<^bsub>X\<^bsup>A\<^esup> \<times>\<^sub>c (B \<setminus> (A, m))\<^esub>) \<circ>\<^sub>c dist_prod_coprod_inv (X\<^bsup>A\<^esup>) A (B \<setminus> (A, m)) \<circ>\<^sub>c swap (A \<Coprod> (B \<setminus> (A, m))) (X\<^bsup>A\<^esup>) \<circ>\<^sub>c try_cast m \<times>\<^sub>f id\<^sub>c (X\<^bsup>A\<^esup>))\<^sup>\<sharp> : X\<^bsup>A\<^esup> \<rightarrow> X\<^bsup>B\<^esup>"
+    show "((eval_func X A \<circ>\<^sub>c swap (X\<^bsup>A\<^esup>) A) \<amalg> (x \<circ>\<^sub>c \<beta>\<^bsub>X\<^bsup>A\<^esup> \<times>\<^sub>c (B \<setminus> (A, m))\<^esub>) \<circ>\<^sub>c dist_prod_coprod_left (X\<^bsup>A\<^esup>) A (B \<setminus> (A, m)) \<circ>\<^sub>c swap (A \<Coprod> (B \<setminus> (A, m))) (X\<^bsup>A\<^esup>) \<circ>\<^sub>c try_cast m \<times>\<^sub>f id\<^sub>c (X\<^bsup>A\<^esup>))\<^sup>\<sharp> : X\<^bsup>A\<^esup> \<rightarrow> X\<^bsup>B\<^esup>"
       by  typecheck_cfuncs
     then show "monomorphism
       (((eval_func X A \<circ>\<^sub>c swap (X\<^bsup>A\<^esup>) A) \<amalg> (x \<circ>\<^sub>c \<beta>\<^bsub>X\<^bsup>A\<^esup> \<times>\<^sub>c (B \<setminus> (A, m))\<^esub>) \<circ>\<^sub>c
-        dist_prod_coprod_inv (X\<^bsup>A\<^esup>) A (B \<setminus> (A, m)) \<circ>\<^sub>c
+        dist_prod_coprod_left (X\<^bsup>A\<^esup>) A (B \<setminus> (A, m)) \<circ>\<^sub>c
         swap (A \<Coprod> (B \<setminus> (A, m))) (X\<^bsup>A\<^esup>) \<circ>\<^sub>c try_cast m \<times>\<^sub>f id\<^sub>c (X\<^bsup>A\<^esup>))\<^sup>\<sharp>)"
     proof (unfold monomorphism_def3, auto)
       fix g h Z
       assume g_type[type_rule]: "g : Z \<rightarrow> X\<^bsup>A\<^esup>"
       assume h_type[type_rule]: "h : Z \<rightarrow> X\<^bsup>A\<^esup>"
       assume eq: "((eval_func X A \<circ>\<^sub>c swap (X\<^bsup>A\<^esup>) A) \<amalg> (x \<circ>\<^sub>c \<beta>\<^bsub>X\<^bsup>A\<^esup> \<times>\<^sub>c (B \<setminus> (A, m))\<^esub>) \<circ>\<^sub>c
-          dist_prod_coprod_inv (X\<^bsup>A\<^esup>) A (B \<setminus> (A, m)) \<circ>\<^sub>c
+          dist_prod_coprod_left (X\<^bsup>A\<^esup>) A (B \<setminus> (A, m)) \<circ>\<^sub>c
           swap (A \<Coprod> (B \<setminus> (A, m))) (X\<^bsup>A\<^esup>) \<circ>\<^sub>c try_cast m \<times>\<^sub>f id\<^sub>c (X\<^bsup>A\<^esup>))\<^sup>\<sharp> \<circ>\<^sub>c g
         =
           ((eval_func X A \<circ>\<^sub>c swap (X\<^bsup>A\<^esup>) A) \<amalg> (x \<circ>\<^sub>c \<beta>\<^bsub>X\<^bsup>A\<^esup> \<times>\<^sub>c (B \<setminus> (A, m))\<^esub>) \<circ>\<^sub>c
-          dist_prod_coprod_inv (X\<^bsup>A\<^esup>) A (B \<setminus> (A, m)) \<circ>\<^sub>c
+          dist_prod_coprod_left (X\<^bsup>A\<^esup>) A (B \<setminus> (A, m)) \<circ>\<^sub>c
           swap (A \<Coprod> (B \<setminus> (A, m))) (X\<^bsup>A\<^esup>) \<circ>\<^sub>c try_cast m \<times>\<^sub>f id\<^sub>c (X\<^bsup>A\<^esup>))\<^sup>\<sharp> \<circ>\<^sub>c h"
 
       show "g = h"
@@ -1001,92 +1001,92 @@ proof (unfold is_smaller_than_def)
             using cart_prod_decomp az_type by blast
 
           have "(eval_func X B) \<circ>\<^sub>c (id B \<times>\<^sub>f (((eval_func X A \<circ>\<^sub>c swap (X\<^bsup>A\<^esup>) A) \<amalg> (x \<circ>\<^sub>c \<beta>\<^bsub>X\<^bsup>A\<^esup> \<times>\<^sub>c (B \<setminus> (A, m))\<^esub>) \<circ>\<^sub>c
-            dist_prod_coprod_inv (X\<^bsup>A\<^esup>) A (B \<setminus> (A, m)) \<circ>\<^sub>c
+            dist_prod_coprod_left (X\<^bsup>A\<^esup>) A (B \<setminus> (A, m)) \<circ>\<^sub>c
             swap (A \<Coprod> (B \<setminus> (A, m))) (X\<^bsup>A\<^esup>) \<circ>\<^sub>c try_cast m \<times>\<^sub>f id\<^sub>c (X\<^bsup>A\<^esup>))\<^sup>\<sharp> \<circ>\<^sub>c g)) = 
           (eval_func X B) \<circ>\<^sub>c (id B \<times>\<^sub>f (((eval_func X A \<circ>\<^sub>c swap (X\<^bsup>A\<^esup>) A) \<amalg> (x \<circ>\<^sub>c \<beta>\<^bsub>X\<^bsup>A\<^esup> \<times>\<^sub>c (B \<setminus> (A, m))\<^esub>) \<circ>\<^sub>c
-            dist_prod_coprod_inv (X\<^bsup>A\<^esup>) A (B \<setminus> (A, m)) \<circ>\<^sub>c
+            dist_prod_coprod_left (X\<^bsup>A\<^esup>) A (B \<setminus> (A, m)) \<circ>\<^sub>c
             swap (A \<Coprod> (B \<setminus> (A, m))) (X\<^bsup>A\<^esup>) \<circ>\<^sub>c try_cast m \<times>\<^sub>f id\<^sub>c (X\<^bsup>A\<^esup>))\<^sup>\<sharp> \<circ>\<^sub>c h))"
             using eq by simp
           then have "(eval_func X B)\<circ>\<^sub>c (id B \<times>\<^sub>f (((eval_func X A \<circ>\<^sub>c swap (X\<^bsup>A\<^esup>) A) \<amalg> (x \<circ>\<^sub>c \<beta>\<^bsub>X\<^bsup>A\<^esup> \<times>\<^sub>c (B \<setminus> (A, m))\<^esub>) \<circ>\<^sub>c
-            dist_prod_coprod_inv (X\<^bsup>A\<^esup>) A (B \<setminus> (A, m)) \<circ>\<^sub>c
+            dist_prod_coprod_left (X\<^bsup>A\<^esup>) A (B \<setminus> (A, m)) \<circ>\<^sub>c
             swap (A \<Coprod> (B \<setminus> (A, m))) (X\<^bsup>A\<^esup>) \<circ>\<^sub>c try_cast m \<times>\<^sub>f id\<^sub>c (X\<^bsup>A\<^esup>))\<^sup>\<sharp>)) \<circ>\<^sub>c (id B \<times>\<^sub>f  g) = 
           (eval_func X B)\<circ>\<^sub>c (id B \<times>\<^sub>f (((eval_func X A \<circ>\<^sub>c swap (X\<^bsup>A\<^esup>) A) \<amalg> (x \<circ>\<^sub>c \<beta>\<^bsub>X\<^bsup>A\<^esup> \<times>\<^sub>c (B \<setminus> (A, m))\<^esub>) \<circ>\<^sub>c
-            dist_prod_coprod_inv (X\<^bsup>A\<^esup>) A (B \<setminus> (A, m)) \<circ>\<^sub>c
+            dist_prod_coprod_left (X\<^bsup>A\<^esup>) A (B \<setminus> (A, m)) \<circ>\<^sub>c
             swap (A \<Coprod> (B \<setminus> (A, m))) (X\<^bsup>A\<^esup>) \<circ>\<^sub>c try_cast m \<times>\<^sub>f id\<^sub>c (X\<^bsup>A\<^esup>))\<^sup>\<sharp>)) \<circ>\<^sub>c (id B \<times>\<^sub>f  h)"
             using identity_distributes_across_composition by (typecheck_cfuncs, auto)
           then have "((eval_func X B)\<circ>\<^sub>c (id B \<times>\<^sub>f (((eval_func X A \<circ>\<^sub>c swap (X\<^bsup>A\<^esup>) A) \<amalg> (x \<circ>\<^sub>c \<beta>\<^bsub>X\<^bsup>A\<^esup> \<times>\<^sub>c (B \<setminus> (A, m))\<^esub>) \<circ>\<^sub>c
-            dist_prod_coprod_inv (X\<^bsup>A\<^esup>) A (B \<setminus> (A, m)) \<circ>\<^sub>c
+            dist_prod_coprod_left (X\<^bsup>A\<^esup>) A (B \<setminus> (A, m)) \<circ>\<^sub>c
             swap (A \<Coprod> (B \<setminus> (A, m))) (X\<^bsup>A\<^esup>) \<circ>\<^sub>c try_cast m \<times>\<^sub>f id\<^sub>c (X\<^bsup>A\<^esup>))\<^sup>\<sharp>))) \<circ>\<^sub>c (id B \<times>\<^sub>f  g) = 
           ((eval_func X B)\<circ>\<^sub>c (id B \<times>\<^sub>f (((eval_func X A \<circ>\<^sub>c swap (X\<^bsup>A\<^esup>) A) \<amalg> (x \<circ>\<^sub>c \<beta>\<^bsub>X\<^bsup>A\<^esup> \<times>\<^sub>c (B \<setminus> (A, m))\<^esub>) \<circ>\<^sub>c
-            dist_prod_coprod_inv (X\<^bsup>A\<^esup>) A (B \<setminus> (A, m)) \<circ>\<^sub>c
+            dist_prod_coprod_left (X\<^bsup>A\<^esup>) A (B \<setminus> (A, m)) \<circ>\<^sub>c
             swap (A \<Coprod> (B \<setminus> (A, m))) (X\<^bsup>A\<^esup>) \<circ>\<^sub>c try_cast m \<times>\<^sub>f id\<^sub>c (X\<^bsup>A\<^esup>))\<^sup>\<sharp>))) \<circ>\<^sub>c (id B \<times>\<^sub>f  h)"
             by (typecheck_cfuncs, smt eq inv_transpose_func_def3 inv_transpose_of_composition)
           then have "((eval_func X A \<circ>\<^sub>c swap (X\<^bsup>A\<^esup>) A) \<amalg> (x \<circ>\<^sub>c \<beta>\<^bsub>X\<^bsup>A\<^esup> \<times>\<^sub>c (B \<setminus> (A, m))\<^esub>) \<circ>\<^sub>c
-            dist_prod_coprod_inv (X\<^bsup>A\<^esup>) A (B \<setminus> (A, m)) \<circ>\<^sub>c
+            dist_prod_coprod_left (X\<^bsup>A\<^esup>) A (B \<setminus> (A, m)) \<circ>\<^sub>c
             swap (A \<Coprod> (B \<setminus> (A, m))) (X\<^bsup>A\<^esup>) \<circ>\<^sub>c try_cast m \<times>\<^sub>f id\<^sub>c (X\<^bsup>A\<^esup>)) \<circ>\<^sub>c (id B \<times>\<^sub>f  g)
           = ((eval_func X A \<circ>\<^sub>c swap (X\<^bsup>A\<^esup>) A) \<amalg> (x \<circ>\<^sub>c \<beta>\<^bsub>X\<^bsup>A\<^esup> \<times>\<^sub>c (B \<setminus> (A, m))\<^esub>) \<circ>\<^sub>c
-            dist_prod_coprod_inv (X\<^bsup>A\<^esup>) A (B \<setminus> (A, m)) \<circ>\<^sub>c
+            dist_prod_coprod_left (X\<^bsup>A\<^esup>) A (B \<setminus> (A, m)) \<circ>\<^sub>c
             swap (A \<Coprod> (B \<setminus> (A, m))) (X\<^bsup>A\<^esup>) \<circ>\<^sub>c try_cast m \<times>\<^sub>f id\<^sub>c (X\<^bsup>A\<^esup>)) \<circ>\<^sub>c (id B \<times>\<^sub>f  h)"
             using   transpose_func_def by (typecheck_cfuncs,auto)
           then have "(((eval_func X A \<circ>\<^sub>c swap (X\<^bsup>A\<^esup>) A) \<amalg> (x \<circ>\<^sub>c \<beta>\<^bsub>X\<^bsup>A\<^esup> \<times>\<^sub>c (B \<setminus> (A, m))\<^esub>) \<circ>\<^sub>c
-            dist_prod_coprod_inv (X\<^bsup>A\<^esup>) A (B \<setminus> (A, m)) \<circ>\<^sub>c
+            dist_prod_coprod_left (X\<^bsup>A\<^esup>) A (B \<setminus> (A, m)) \<circ>\<^sub>c
             swap (A \<Coprod> (B \<setminus> (A, m))) (X\<^bsup>A\<^esup>) \<circ>\<^sub>c try_cast m \<times>\<^sub>f id\<^sub>c (X\<^bsup>A\<^esup>)) \<circ>\<^sub>c (id B \<times>\<^sub>f  g)) \<circ>\<^sub>c \<langle>m \<circ>\<^sub>c a, z\<rangle>
           = (((eval_func X A \<circ>\<^sub>c swap (X\<^bsup>A\<^esup>) A) \<amalg> (x \<circ>\<^sub>c \<beta>\<^bsub>X\<^bsup>A\<^esup> \<times>\<^sub>c (B \<setminus> (A, m))\<^esub>) \<circ>\<^sub>c
-            dist_prod_coprod_inv (X\<^bsup>A\<^esup>) A (B \<setminus> (A, m)) \<circ>\<^sub>c
+            dist_prod_coprod_left (X\<^bsup>A\<^esup>) A (B \<setminus> (A, m)) \<circ>\<^sub>c
             swap (A \<Coprod> (B \<setminus> (A, m))) (X\<^bsup>A\<^esup>) \<circ>\<^sub>c try_cast m \<times>\<^sub>f id\<^sub>c (X\<^bsup>A\<^esup>)) \<circ>\<^sub>c (id B \<times>\<^sub>f  h)) \<circ>\<^sub>c \<langle>m \<circ>\<^sub>c a, z\<rangle>"
             by auto
           then have "((eval_func X A \<circ>\<^sub>c swap (X\<^bsup>A\<^esup>) A) \<amalg> (x \<circ>\<^sub>c \<beta>\<^bsub>X\<^bsup>A\<^esup> \<times>\<^sub>c (B \<setminus> (A, m))\<^esub>) \<circ>\<^sub>c
-            dist_prod_coprod_inv (X\<^bsup>A\<^esup>) A (B \<setminus> (A, m)) \<circ>\<^sub>c
+            dist_prod_coprod_left (X\<^bsup>A\<^esup>) A (B \<setminus> (A, m)) \<circ>\<^sub>c
             swap (A \<Coprod> (B \<setminus> (A, m))) (X\<^bsup>A\<^esup>) \<circ>\<^sub>c try_cast m \<times>\<^sub>f id\<^sub>c (X\<^bsup>A\<^esup>)) \<circ>\<^sub>c (id B \<times>\<^sub>f  g) \<circ>\<^sub>c \<langle>m \<circ>\<^sub>c a, z\<rangle>
           = ((eval_func X A \<circ>\<^sub>c swap (X\<^bsup>A\<^esup>) A) \<amalg> (x \<circ>\<^sub>c \<beta>\<^bsub>X\<^bsup>A\<^esup> \<times>\<^sub>c (B \<setminus> (A, m))\<^esub>) \<circ>\<^sub>c
-            dist_prod_coprod_inv (X\<^bsup>A\<^esup>) A (B \<setminus> (A, m)) \<circ>\<^sub>c
+            dist_prod_coprod_left (X\<^bsup>A\<^esup>) A (B \<setminus> (A, m)) \<circ>\<^sub>c
             swap (A \<Coprod> (B \<setminus> (A, m))) (X\<^bsup>A\<^esup>) \<circ>\<^sub>c try_cast m \<times>\<^sub>f id\<^sub>c (X\<^bsup>A\<^esup>)) \<circ>\<^sub>c (id B \<times>\<^sub>f  h) \<circ>\<^sub>c \<langle>m \<circ>\<^sub>c a, z\<rangle>"
             by (typecheck_cfuncs, auto simp add: comp_associative2)
           then have "((eval_func X A \<circ>\<^sub>c swap (X\<^bsup>A\<^esup>) A) \<amalg> (x \<circ>\<^sub>c \<beta>\<^bsub>X\<^bsup>A\<^esup> \<times>\<^sub>c (B \<setminus> (A, m))\<^esub>) \<circ>\<^sub>c
-            dist_prod_coprod_inv (X\<^bsup>A\<^esup>) A (B \<setminus> (A, m)) \<circ>\<^sub>c
+            dist_prod_coprod_left (X\<^bsup>A\<^esup>) A (B \<setminus> (A, m)) \<circ>\<^sub>c
             swap (A \<Coprod> (B \<setminus> (A, m))) (X\<^bsup>A\<^esup>) \<circ>\<^sub>c try_cast m \<times>\<^sub>f id\<^sub>c (X\<^bsup>A\<^esup>)) \<circ>\<^sub>c \<langle>m \<circ>\<^sub>c a, g \<circ>\<^sub>c z\<rangle>
           = ((eval_func X A \<circ>\<^sub>c swap (X\<^bsup>A\<^esup>) A) \<amalg> (x \<circ>\<^sub>c \<beta>\<^bsub>X\<^bsup>A\<^esup> \<times>\<^sub>c (B \<setminus> (A, m))\<^esub>) \<circ>\<^sub>c
-            dist_prod_coprod_inv (X\<^bsup>A\<^esup>) A (B \<setminus> (A, m)) \<circ>\<^sub>c
+            dist_prod_coprod_left (X\<^bsup>A\<^esup>) A (B \<setminus> (A, m)) \<circ>\<^sub>c
             swap (A \<Coprod> (B \<setminus> (A, m))) (X\<^bsup>A\<^esup>) \<circ>\<^sub>c try_cast m \<times>\<^sub>f id\<^sub>c (X\<^bsup>A\<^esup>)) \<circ>\<^sub>c \<langle>m \<circ>\<^sub>c a, h \<circ>\<^sub>c z\<rangle>"
             by (typecheck_cfuncs, smt cfunc_cross_prod_comp_cfunc_prod id_left_unit2 id_type)
           then have "(eval_func X A \<circ>\<^sub>c swap (X\<^bsup>A\<^esup>) A) \<amalg> (x \<circ>\<^sub>c \<beta>\<^bsub>X\<^bsup>A\<^esup> \<times>\<^sub>c (B \<setminus> (A, m))\<^esub>) \<circ>\<^sub>c
-            dist_prod_coprod_inv (X\<^bsup>A\<^esup>) A (B \<setminus> (A, m)) \<circ>\<^sub>c
+            dist_prod_coprod_left (X\<^bsup>A\<^esup>) A (B \<setminus> (A, m)) \<circ>\<^sub>c
             swap (A \<Coprod> (B \<setminus> (A, m))) (X\<^bsup>A\<^esup>) \<circ>\<^sub>c (try_cast m \<times>\<^sub>f id\<^sub>c (X\<^bsup>A\<^esup>)) \<circ>\<^sub>c \<langle>m \<circ>\<^sub>c a, g \<circ>\<^sub>c z\<rangle>
           = (eval_func X A \<circ>\<^sub>c swap (X\<^bsup>A\<^esup>) A) \<amalg> (x \<circ>\<^sub>c \<beta>\<^bsub>X\<^bsup>A\<^esup> \<times>\<^sub>c (B \<setminus> (A, m))\<^esub>) \<circ>\<^sub>c
-            dist_prod_coprod_inv (X\<^bsup>A\<^esup>) A (B \<setminus> (A, m)) \<circ>\<^sub>c
+            dist_prod_coprod_left (X\<^bsup>A\<^esup>) A (B \<setminus> (A, m)) \<circ>\<^sub>c
             swap (A \<Coprod> (B \<setminus> (A, m))) (X\<^bsup>A\<^esup>) \<circ>\<^sub>c (try_cast m \<times>\<^sub>f id\<^sub>c (X\<^bsup>A\<^esup>)) \<circ>\<^sub>c \<langle>m \<circ>\<^sub>c a, h \<circ>\<^sub>c z\<rangle>"
             by (typecheck_cfuncs_prems, smt comp_associative2)
           then have "(eval_func X A \<circ>\<^sub>c swap (X\<^bsup>A\<^esup>) A) \<amalg> (x \<circ>\<^sub>c \<beta>\<^bsub>X\<^bsup>A\<^esup> \<times>\<^sub>c (B \<setminus> (A, m))\<^esub>) \<circ>\<^sub>c
-            dist_prod_coprod_inv (X\<^bsup>A\<^esup>) A (B \<setminus> (A, m)) \<circ>\<^sub>c
+            dist_prod_coprod_left (X\<^bsup>A\<^esup>) A (B \<setminus> (A, m)) \<circ>\<^sub>c
             swap (A \<Coprod> (B \<setminus> (A, m))) (X\<^bsup>A\<^esup>) \<circ>\<^sub>c \<langle>try_cast m \<circ>\<^sub>c m \<circ>\<^sub>c a, g \<circ>\<^sub>c z\<rangle>
           = (eval_func X A \<circ>\<^sub>c swap (X\<^bsup>A\<^esup>) A) \<amalg> (x \<circ>\<^sub>c \<beta>\<^bsub>X\<^bsup>A\<^esup> \<times>\<^sub>c (B \<setminus> (A, m))\<^esub>) \<circ>\<^sub>c
-            dist_prod_coprod_inv (X\<^bsup>A\<^esup>) A (B \<setminus> (A, m)) \<circ>\<^sub>c
+            dist_prod_coprod_left (X\<^bsup>A\<^esup>) A (B \<setminus> (A, m)) \<circ>\<^sub>c
             swap (A \<Coprod> (B \<setminus> (A, m))) (X\<^bsup>A\<^esup>) \<circ>\<^sub>c \<langle>try_cast m \<circ>\<^sub>c m \<circ>\<^sub>c a, h \<circ>\<^sub>c z\<rangle>"
             using cfunc_cross_prod_comp_cfunc_prod id_left_unit2 by (typecheck_cfuncs_prems, smt)
           then have "(eval_func X A \<circ>\<^sub>c swap (X\<^bsup>A\<^esup>) A) \<amalg> (x \<circ>\<^sub>c \<beta>\<^bsub>X\<^bsup>A\<^esup> \<times>\<^sub>c (B \<setminus> (A, m))\<^esub>) \<circ>\<^sub>c
-            dist_prod_coprod_inv (X\<^bsup>A\<^esup>) A (B \<setminus> (A, m)) \<circ>\<^sub>c
+            dist_prod_coprod_left (X\<^bsup>A\<^esup>) A (B \<setminus> (A, m)) \<circ>\<^sub>c
             swap (A \<Coprod> (B \<setminus> (A, m))) (X\<^bsup>A\<^esup>) \<circ>\<^sub>c \<langle>(try_cast m \<circ>\<^sub>c m) \<circ>\<^sub>c a, g \<circ>\<^sub>c z\<rangle>
           = (eval_func X A \<circ>\<^sub>c swap (X\<^bsup>A\<^esup>) A) \<amalg> (x \<circ>\<^sub>c \<beta>\<^bsub>X\<^bsup>A\<^esup> \<times>\<^sub>c (B \<setminus> (A, m))\<^esub>) \<circ>\<^sub>c
-            dist_prod_coprod_inv (X\<^bsup>A\<^esup>) A (B \<setminus> (A, m)) \<circ>\<^sub>c
+            dist_prod_coprod_left (X\<^bsup>A\<^esup>) A (B \<setminus> (A, m)) \<circ>\<^sub>c
             swap (A \<Coprod> (B \<setminus> (A, m))) (X\<^bsup>A\<^esup>) \<circ>\<^sub>c \<langle>(try_cast m \<circ>\<^sub>c m) \<circ>\<^sub>c a, h \<circ>\<^sub>c z\<rangle>"
             by (typecheck_cfuncs, auto simp add: comp_associative2)
           then have "(eval_func X A \<circ>\<^sub>c swap (X\<^bsup>A\<^esup>) A) \<amalg> (x \<circ>\<^sub>c \<beta>\<^bsub>X\<^bsup>A\<^esup> \<times>\<^sub>c (B \<setminus> (A, m))\<^esub>) \<circ>\<^sub>c
-            dist_prod_coprod_inv (X\<^bsup>A\<^esup>) A (B \<setminus> (A, m)) \<circ>\<^sub>c
+            dist_prod_coprod_left (X\<^bsup>A\<^esup>) A (B \<setminus> (A, m)) \<circ>\<^sub>c
             swap (A \<Coprod> (B \<setminus> (A, m))) (X\<^bsup>A\<^esup>) \<circ>\<^sub>c \<langle>left_coproj A (B \<setminus> (A,m)) \<circ>\<^sub>c a, g \<circ>\<^sub>c z\<rangle>
           = (eval_func X A \<circ>\<^sub>c swap (X\<^bsup>A\<^esup>) A) \<amalg> (x \<circ>\<^sub>c \<beta>\<^bsub>X\<^bsup>A\<^esup> \<times>\<^sub>c (B \<setminus> (A, m))\<^esub>) \<circ>\<^sub>c
-            dist_prod_coprod_inv (X\<^bsup>A\<^esup>) A (B \<setminus> (A, m)) \<circ>\<^sub>c
+            dist_prod_coprod_left (X\<^bsup>A\<^esup>) A (B \<setminus> (A, m)) \<circ>\<^sub>c
             swap (A \<Coprod> (B \<setminus> (A, m))) (X\<^bsup>A\<^esup>) \<circ>\<^sub>c \<langle>left_coproj A (B \<setminus> (A,m)) \<circ>\<^sub>c a, h \<circ>\<^sub>c z\<rangle>"
             using m_def(2) try_cast_m_m by (typecheck_cfuncs, auto)
           then have "(eval_func X A \<circ>\<^sub>c swap (X\<^bsup>A\<^esup>) A) \<amalg> (x \<circ>\<^sub>c \<beta>\<^bsub>X\<^bsup>A\<^esup> \<times>\<^sub>c (B \<setminus> (A, m))\<^esub>) \<circ>\<^sub>c
-            dist_prod_coprod_inv (X\<^bsup>A\<^esup>) A (B \<setminus> (A, m)) \<circ>\<^sub>c \<langle>g \<circ>\<^sub>c z, left_coproj A (B \<setminus> (A,m)) \<circ>\<^sub>c a\<rangle>
+            dist_prod_coprod_left (X\<^bsup>A\<^esup>) A (B \<setminus> (A, m)) \<circ>\<^sub>c \<langle>g \<circ>\<^sub>c z, left_coproj A (B \<setminus> (A,m)) \<circ>\<^sub>c a\<rangle>
           = (eval_func X A \<circ>\<^sub>c swap (X\<^bsup>A\<^esup>) A) \<amalg> (x \<circ>\<^sub>c \<beta>\<^bsub>X\<^bsup>A\<^esup> \<times>\<^sub>c (B \<setminus> (A, m))\<^esub>) \<circ>\<^sub>c
-            dist_prod_coprod_inv (X\<^bsup>A\<^esup>) A (B \<setminus> (A, m)) \<circ>\<^sub>c \<langle>h \<circ>\<^sub>c z, left_coproj A (B \<setminus> (A,m)) \<circ>\<^sub>c a\<rangle>"
+            dist_prod_coprod_left (X\<^bsup>A\<^esup>) A (B \<setminus> (A, m)) \<circ>\<^sub>c \<langle>h \<circ>\<^sub>c z, left_coproj A (B \<setminus> (A,m)) \<circ>\<^sub>c a\<rangle>"
             using swap_ap by (typecheck_cfuncs, auto)
           then have "(eval_func X A \<circ>\<^sub>c swap (X\<^bsup>A\<^esup>) A) \<amalg> (x \<circ>\<^sub>c \<beta>\<^bsub>X\<^bsup>A\<^esup> \<times>\<^sub>c (B \<setminus> (A, m))\<^esub>) \<circ>\<^sub>c
             left_coproj (X\<^bsup>A\<^esup>\<times>\<^sub>cA) (X\<^bsup>A\<^esup>\<times>\<^sub>c(B \<setminus> (A,m))) \<circ>\<^sub>c \<langle>g \<circ>\<^sub>c z, a\<rangle>
           = (eval_func X A \<circ>\<^sub>c swap (X\<^bsup>A\<^esup>) A) \<amalg> (x \<circ>\<^sub>c \<beta>\<^bsub>X\<^bsup>A\<^esup> \<times>\<^sub>c (B \<setminus> (A, m))\<^esub>) \<circ>\<^sub>c
             left_coproj (X\<^bsup>A\<^esup>\<times>\<^sub>cA) (X\<^bsup>A\<^esup>\<times>\<^sub>c(B \<setminus> (A,m))) \<circ>\<^sub>c \<langle>h \<circ>\<^sub>c z,a\<rangle>"
-            using dist_prod_coprod_inv_left_ap by (typecheck_cfuncs, auto)
+            using dist_prod_coprod_left_ap_left by (typecheck_cfuncs, auto)
           then have "((eval_func X A \<circ>\<^sub>c swap (X\<^bsup>A\<^esup>) A) \<amalg> (x \<circ>\<^sub>c \<beta>\<^bsub>X\<^bsup>A\<^esup> \<times>\<^sub>c (B \<setminus> (A, m))\<^esub>) \<circ>\<^sub>c
             left_coproj (X\<^bsup>A\<^esup>\<times>\<^sub>cA) (X\<^bsup>A\<^esup>\<times>\<^sub>c(B \<setminus> (A,m)))) \<circ>\<^sub>c \<langle>g \<circ>\<^sub>c z, a\<rangle>
           = ((eval_func X A \<circ>\<^sub>c swap (X\<^bsup>A\<^esup>) A) \<amalg> (x \<circ>\<^sub>c \<beta>\<^bsub>X\<^bsup>A\<^esup> \<times>\<^sub>c (B \<setminus> (A, m))\<^esub>) \<circ>\<^sub>c
