HOL-ETCS/Nat_Parity.thy
@@ -1,8 +1,10 @@
+section \<open>Natural Number Parity and Halving\<close>
+
 theory Nat_Parity
   imports Nats Quant_Logic
 begin
 
-section \<open>Nth Even Number\<close>
+subsection \<open>Nth Even Number\<close>
 
 definition nth_even :: "cfunc" where
   "nth_even = (THE u. u: \<nat>\<^sub>c \<rightarrow> \<nat>\<^sub>c \<and> 
@@ -29,7 +31,7 @@ lemma nth_even_successor2:
   "nth_even \<circ>\<^sub>c successor = successor \<circ>\<^sub>c successor \<circ>\<^sub>c nth_even"
   using comp_associative2 nth_even_def2 by (typecheck_cfuncs, auto)
 
-section \<open>Nth Odd Number\<close>
+subsection \<open>Nth Odd Number\<close>
 
 definition nth_odd :: "cfunc" where
   "nth_odd = (THE u. u: \<nat>\<^sub>c \<rightarrow> \<nat>\<^sub>c \<and> 
@@ -117,7 +119,7 @@ proof (rule natural_number_object_func_unique[where X="\<nat>\<^sub>c", where f=
     using nth_even_successor2 nth_odd_is_succ_nth_even by auto
 qed
 
-section \<open>Checking if a Number is Even\<close>
+subsection \<open>Checking if a Number is Even\<close>
 
 definition is_even :: "cfunc" where
   "is_even = (THE u. u: \<nat>\<^sub>c \<rightarrow> \<Omega> \<and> u \<circ>\<^sub>c zero = \<t> \<and> NOT \<circ>\<^sub>c u = u \<circ>\<^sub>c successor)"
@@ -138,7 +140,7 @@ lemma is_even_successor:
   "is_even \<circ>\<^sub>c successor = NOT \<circ>\<^sub>c is_even"
   by (simp add: is_even_def2)
 
-section \<open>Checking if a Number is Odd\<close>
+subsection \<open>Checking if a Number is Odd\<close>
 
 definition is_odd :: "cfunc" where
   "is_odd = (THE u. u: \<nat>\<^sub>c \<rightarrow> \<Omega> \<and> u \<circ>\<^sub>c zero = \<f> \<and> NOT \<circ>\<^sub>c u = u \<circ>\<^sub>c successor)"
@@ -369,7 +371,7 @@ proof -
     using calculation by auto
 qed
 
-section \<open>Natural Number Halving\<close>
+subsection \<open>Natural Number Halving\<close>
 
 definition halve_with_parity :: "cfunc" where
   "halve_with_parity = (THE u. u: \<nat>\<^sub>c \<rightarrow> \<nat>\<^sub>c \<Coprod> \<nat>\<^sub>c \<and> 
